Wasm/Compiler.lean
@@ -7,12 +7,18 @@ inductive Expr : ValType -> Type
 | I32Sub (lhs : Expr .I32) (rhs : Expr .I32) : Expr .I32
 | F32Add (lhs : Expr .F32) (rhs : Expr .F32) : Expr .F32
 
-def Expr.eval (e : Expr T) : T.repr := match e with
-| .I32Lit n => n
-| .F32Lit n => n
-| .I32Add lhs rhs => lhs.eval + rhs.eval
-| .I32Sub lhs rhs => lhs.eval - rhs.eval
-| .F32Add lhs rhs => lhs.eval + rhs.eval
+def Expr.eval' (e : Expr T) : TVal T := match e with
+| .I32Lit n => .I32 n
+| .F32Lit n => .F32 n
+| .I32Add lhs rhs => .I32 $ lhs.eval'.toRepr + rhs.eval'.toRepr
+| .I32Sub lhs rhs => .I32 $ lhs.eval'.toRepr - rhs.eval'.toRepr
+| .F32Add lhs rhs => .F32 $ lhs.eval'.toRepr + rhs.eval'.toRepr
+
+def Expr.eval (e : Expr T) : T.repr := 
+  let tv := e.eval'
+  let ⟨v, h⟩ := tv.toValR
+  have h' : v.toValType.repr = T.repr := by rw [h];
+  h ▸ v.toRepr
 
 def testExpr : Expr .I32 := .I32Add (.I32Lit 5) (.I32Add (.I32Lit 10) (.I32Lit 15))
 def evalRes := testExpr.eval
@@ -64,10 +70,46 @@ theorem eval_nil {st : Stack} {h : st.types = inpTys} : (evalProg' (@Prog.nil in
 /-   subst h; rfl -/
 
 @[simp]
-theorem concat_nil {a b : StackTypes} {lhs : Prog a b} : Prog.concat lhs Prog.nil = lhs := by
+theorem concat_nil_l {a b : StackTypes} {lhs : Prog a b} : Prog.concat lhs Prog.nil = lhs := by
   induction lhs with
   | nil => rfl
   | cons op rest ih => unfold Prog.concat; rw [ih];
+
+@[simp]
+theorem concat_nil_r {a b : StackTypes} {rhs : Prog a b} : Prog.concat Prog.nil rhs = rhs := rfl
+
+/- theorem concat_cons_eval {a b c: StackTypes} -/
+/-   (left : Prog a b) (right : Prog b c) {op : Op b s} {rrest : Prog s c} -/
+/-   (st : Stack) (h : st.types = a) -/
+/-   : (right = Prog.cons op rrest) -> -/
+/-       let ⟨lstack, lh⟩ := evalProg' left st h -/
+/-       let ⟨step, sh⟩ := evalOp' op lstack lh -/
+/-       let ⟨final, rh⟩ := evalProg' rrest step sh -/
+/-       evalProg' (Prog.concat left right) st h = evalProg' rrest step sh -/
+/- := by -/ 
+/-   simp; intro right_def; -/
+/-   induction left with -/
+/-   | nil => unfold evalProg'; simp; cases right with -/
+/-                                    | nil => contradiction; -/
+/-                                    | cons op' rrest' => rw [right_def, ← evalProg'.eq_def]; -/
+/-   | cons l_op lrest ih => unfold evalProg'; simp; cases right with -/
+/-                                                   | nil => contradiction; -/
+/-                                                   | cons op' rrest' => rw [right_def, <- evalProg'.eq_def]; sorry -/
+
+theorem concat_cons_eval {a b c: StackTypes}
+  (left : Prog a b) (op : Op b s) (rrest : Prog s c)
+  (st : Stack) (h : st.types = a)
+  :
+      let ⟨lstack, lh⟩ := evalProg' left st h
+      let ⟨step, sh⟩ := evalOp' op lstack lh
+      let ⟨final, rh⟩ := evalProg' rrest step sh
+      evalProg' (Prog.concat left (op ;; rrest)) st h = evalProg' rrest step sh
+:= by
+  simp; induction rrest with
+  | nil => conv => right; unfold evalProg';
+           conv => left; unfold evalProg' Prog.concat;
+           sorry
+  | cons op rest rest_ih => sorry
 
 theorem concat_eval {a b c : StackTypes} 
   (left : Prog a b) (right : Prog b c) 
@@ -79,7 +121,14 @@ theorem concat_eval {a b c : StackTypes}
   dsimp;
   induction right with
   | nil => aesop
-  | cons r_op rrest r_ih => sorry
+  | cons r_op rrest r_ih =>
+      rw [Subtype.ext_iff];
+      conv => right; unfold evalProg'; dsimp;
+      let ⟨lstack, lh⟩ := evalProg' left astack ah
+      let ⟨step, sh⟩ := evalOp' r_op lstack lh
+      let ⟨final, rh⟩ := evalProg' rrest step sh;
+      /- rw [concat_cons_eval]; -/
+
   /- induction left with -/
   /- | @nil s => -/
   /-     conv => rhs; arg 2; rw [eval_nil]; -/
@@ -102,26 +151,62 @@ theorem concat_eval {a b c : StackTypes}
 
   /-     sorry -/
 
-theorem compile_head_eq_eval : ∀ (e : Expr T), eval_eq_compile e := by
-  intro e; unfold eval_eq_compile; intro prog compile_res; simp;
-  induction e with
-  | I32Lit n =>
-      unfold progResHead;
-      have hc : compile_res = ⟨[Val.I32 n], by simp⟩ := by
-        (unfold compile_res; unfold prog Expr.compile evalProg evalOp evalProg; dsimp)
-      rw [hc]; dsimp; rfl;
-  | F32Lit n =>
-      unfold progResHead;
-      have hc : compile_res = ⟨[Val.F32 n], by simp⟩ := by
-        (unfold compile_res; unfold prog Expr.compile evalProg evalOp evalProg; dsimp)
-      rw [hc]; dsimp;
-      unfold Expr.eval; rfl;
-  | I32Add lhs rhs lhs_ih rhs_ih =>
-      unfold progResHead compile_res;
-      have hc : compile_res = sorry := by (
-        unfold compile_res prog Expr.compile;
-        have : evalProg [] (Prog.concat lhs.compile rhs.compile) = sorry := by (
-          unfold Prog.concat; dsimp; sorry)
+-- TODO: rewrite without progResHead, insteal have smth like (eval e) :: stack
+/- theorem compile_head_eq_eval : ∀ (e : Expr T), eval_eq_compile e := by -/
+/-   intro e; unfold eval_eq_compile; intro prog compile_res; simp; -/
+/-   induction e with -/
+/-   | I32Lit n => -/
+/-       unfold progResHead; -/
+/-       have hc : compile_res = ⟨[Val.I32 n], by simp⟩ := by -/
+/-         (unfold compile_res; unfold prog Expr.compile evalProg evalOp evalProg; dsimp) -/
+/-       rw [hc]; dsimp; rfl; -/
+/-   | F32Lit n => -/
+/-       unfold progResHead; -/
+/-       have hc : compile_res = ⟨[Val.F32 n], by simp⟩ := by -/
+/-         (unfold compile_res; unfold prog Expr.compile evalProg evalOp evalProg; dsimp) -/
+/-       rw [hc]; dsimp; -/
+/-       unfold Expr.eval; rfl; -/
+/-   | I32Add lhs rhs lhs_ih rhs_ih => -/
+/-       have hc : compile_res = sorry := by ( -/
+/-         unfold compile_res prog Expr.compile; -/
+/-         unfold progResHead at *; -/
+
+theorem prog_eval_concat : evalProg' (Prog.concat l r) st h = evalProg' r (evalProg' l st h) h'
+  := by
+    induction l generalizing st with
+    | nil => simp
+    | cons op_l rest_l ihl =>
+        conv => left; unfold Prog.concat evalProg'; simp;
+        rw [ihl]; rfl;
+
+theorem eval_prog_append : evalProg' (Prog.append l op) st h = evalOp' op (evalProg' l st h) h'
+  := by
+    induction l generalizing st with
+    | nil => simp [evalProg']
+    | cons l_op rest ih => simp [evalProg']; rw [ih];
+        
+theorem compile_eq_eval {T : ValType} {stypes : StackTypes} {st : Stack} {h : st.types = stypes}
+  : ∀ (e : Expr T), (evalProg' e.compile st h).val = e.eval'.toVal :: st
+  := by
+      intro e;
+      induction e generalizing st stypes with
+      | I32Lit n => conv => left; simp [evalProg', Expr.compile, evalOp'];
+                    conv => right; simp [Expr.eval', TVal.toVal];
+      | F32Lit n => conv => left; simp [evalProg', Expr.compile, evalOp'];
+                    conv => right; simp [Expr.eval', TVal.toVal];
+      | I32Add lhs rhs ihl ihr =>
+          conv => left; unfold Expr.compile; rw [prog_append_assoc];
+          rw [prog_eval_concat];
+          · conv => left; arg 1; arg 2; rw [ihl];
+            rw [eval_prog_append];
+            rotate_left;
+            -- proving type hypotheses
+            · grind -- idk if this is a good use of grind
+            · grind
+            · conv => left; arg 1; arg 2; rw [ihr];
+              simp [Expr.eval'];
+              -- scuffed here bc of TVal/Val differences :/
+              sorry
   /- have ⟨res, h⟩ := progResHead compile_res; -/
   /- have h' : T.repr = res.toValType.repr := by rw [h]; -/
   /- show (res.toRepr = h' ▸ e.eval); -/
